# baseURI: https://w3id.org/isample/opencontext/materialsampleobjecttype/0.1/oc_msotvocab
# imports: http://www.w3.org/2004/02/skos/core

@prefix dcterms: <http://purl.org/dc/terms/> .
@prefix msot: <https://w3id.org/isample/vocabulary/materialsampleobjecttype/1.0/> .
@prefix ocmsot: <https://w3id.org/isample/opencontext/materialsampleobjecttype/0.1/> .
@prefix owl: <http://www.w3.org/2002/07/owl#> .
@prefix rdf: <http://www.w3.org/1999/02/22-rdf-syntax-ns#> .
@prefix rdfs: <http://www.w3.org/2000/01/rdf-schema#> .
@prefix schema: <http://schema.org/> .
@prefix skos: <http://www.w3.org/2004/02/skos/core#> .
@prefix xsd: <http://www.w3.org/2001/XMLSchema#> .

<AWDID:2004562>
  rdf:type schema:Grant ;
  schema:funder <https://ror.org/04nh1dc89> ;
  schema:name "Collaborative Research: Frameworks: Internet of Samples: Toward an Interdisciplinary Cyberinfrastructure for Material Samples" ;
  schema:url "https://nsf.gov/awardsearch/showAward?AWD_ID=2004562" ;
.
ocmsot:architecturalelement
  rdf:type skos:Concept ;
  rdfs:label "Architectural element"@en ;
  skos:broader msot:artifact ;
  skos:definition "Artifact that was part of a building."@en ;
  skos:example "akroterion, antefix, finial, moulding, sima, blocks (shaped masses), brick, building stone, stud"@en ;
  skos:inScheme ocmsot:oc_msotvocab ;
  skos:note "could be subdivided into structural (e.g. brick, building stone, stud), ornamental (antefix, finial, moulding), and utilitarian (rainwater-spout, ridge-tile, roof-tile, window-pane) ?"@en ;
  skos:prefLabel "Architectural element"@en ;
.
ocmsot:clothing
  rdf:type skos:Concept ;
  rdfs:label "Clothing"@en ;
  skos:broader msot:artifact ;
  skos:definition "Item intended to be worn to cover the (human) body"@en ;
  skos:example "shoes (footwear), shirt, jacket, pants, skirt, cape"@en ;
  skos:inScheme ocmsot:oc_msotvocab ;
  skos:note "Includes parts of clothing objects like buttons (fasteners), color patches (military patches), buckles, but not external decorations (jewlery, ornamental brooches)."@en ;
  skos:prefLabel "Clothing"@en ;
.
ocmsot:coin
  rdf:type skos:Concept ;
  rdfs:label "Coin"@en ;
  skos:broader msot:artifact ;
  skos:definition "peice of metal issued by some authority and recognized as money."@en ;
  skos:inScheme ocmsot:oc_msotvocab ;
  skos:note "Typically flat, with some identifying feature imprinted on the surface to establish authenticity and value"@en ;
  skos:prefLabel "Coin"@en ;
.
ocmsot:containerobject
  rdf:type skos:Concept ;
  rdfs:label "Container object"@en ;
  skos:broader msot:artifact ;
  skos:definition "Item designed to contain some fluid, granular material, or other items for preservation, transportation or display."@en ;
  skos:example "amphora, aryballos, barrel, bottle, jar, Oenochoe, pithos"@en ;
  skos:inScheme ocmsot:oc_msotvocab ;
  skos:prefLabel "Container object"@en ;
.
ocmsot:domesticitem
  rdf:type skos:Concept ;
  rdfs:label "Domestic item"@en ;
  skos:broader msot:artifact ;
  skos:definition "item intended for household use."@en ;
  skos:example "loom weight, needle, spindle-whorl, spool, cup, dish, plate, cooking-pan, cooking-stand, funnel, grinding-stone, lid, stoneware (pottery), utensils, globes (lighting device components), lamp, cosmetic-pot"@en ;
  skos:inScheme ocmsot:oc_msotvocab ;
  skos:prefLabel "Domestic item"@en ;
.
ocmsot:oc_msotvocab
  rdf:type owl:Ontology ;
  rdf:type skos:ConceptScheme ;
  dcterms:contributor "Hong Cui, Sarah Hyunju Song" ;
  dcterms:created "2022-09-30"^^xsd:date ;
  dcterms:creator <https://orcid.org/0000-0001-6041-5302> ;
  dcterms:license <https://creativecommons.org/licenses/by/4.0/legalcode> ;
  schema:codeRepository <https://github.com/isamplesorg/metadata_profile_archaeology/tree/main/vocabulary> ;
  schema:funding <AWDID:2004562> ;
  schema:provider <http://cor.esipfed.org/ont#/> ;
  rdfs:comment "Vocabulary created based on summary of 'type' values found in OpenContext sample descriptions. This is a bottom-up vocabulary intended as a first draft and demonstration of a material sample type extension for the Open Context community in the iSamples context. Most of the categories are subclasses of msot:Artifact, except for 'bone object' which is a msot:OrganismPart."@en ;
  rdfs:label "Open Context vocabulary extension for material sample object type"@en ;
  owl:imports <http://www.w3.org/2004/02/skos/core> ;
  skos:definition "categories for kinds of sample objects specific to archaeological studies"@en ;
  skos:inScheme msot:materialsampleobjecttypevocabulary ;
  skos:prefLabel "Open Context vocabulary extension for material sample object type"@en ;
.
ocmsot:ornament
  rdf:type skos:Concept ;
  rdfs:label "Ornament"@en ;
  skos:broader msot:artifact ;
  skos:definition "item intended for decoration."@en ;
  skos:example "bead, pendant, ring, inlay, plaque, statuette, tondo"@en ;
  skos:inScheme ocmsot:oc_msotvocab ;
  skos:prefLabel "Ornament"@en ;
.
ocmsot:peiceofbone
  rdf:type skos:Concept ;
  rdfs:label "Bone object"@en ;
  skos:broader msot:organismpart ;
  skos:definition "Sample is an individual bone or part of a bone from an animal."@en ;
  skos:inScheme ocmsot:oc_msotvocab ;
  skos:prefLabel "Bone object"@en ;
.
ocmsot:photograph
  rdf:type skos:Concept ;
  rdfs:label "Photograph"@en ;
  skos:broader msot:artifact ;
  skos:definition "image produced by the action of light on a chemically sensitive surface, preserved on paper, glass or other physical substrate."@en ;
  skos:inScheme ocmsot:oc_msotvocab ;
  skos:note "in this context, photograph is the physical object manifesting the image, not the image itself, which can also be represented electronically"@en ;
  skos:prefLabel "Photograph"@en ;
.
ocmsot:sherd
  rdf:type skos:Concept ;
  rdfs:label "Pot sherd"@en ;
  skos:broader msot:artifact ;
  skos:definition "fragment of pottery"@en ;
  skos:inScheme ocmsot:oc_msotvocab ;
  skos:prefLabel "Pot sherd"@en ;
.
ocmsot:tile
  rdf:type skos:Concept ;
  rdfs:label "Tile"@en ;
  skos:broader msot:artifact ;
  skos:definition "flat or curved piece of fired clay, stone, or concrete used especially for roofs, floors, or walls and often for ornamental work"@en ;
  skos:inScheme ocmsot:oc_msotvocab ;
  skos:note "note possible overlap with 'Architectural element' and 'Ornament'"@en ;
  skos:prefLabel "Tile"@en ;
.
ocmsot:utilityitem
  rdf:type skos:Concept ;
  rdfs:label "Utility item"@en ;
  skos:broader msot:artifact ;
  skos:definition "Item intended for use in manufacture, construction, agriculture or other work activity."@en ;
  skos:example "bolts (fasteners), hooks (fasteners), nails (fasteners), rivet, screws, spike, bellows, chain, crucible, stamps (tools), wire, tools"@en ;
  skos:inScheme ocmsot:oc_msotvocab ;
  skos:prefLabel "Utility item"@en ;
.
ocmsot:weapon
  rdf:type skos:Concept ;
  rdfs:label "Weapon"@en ;
  skos:broader msot:artifact ;
  skos:definition "Item for use in combat, hunting, or self defense"@en ;
  skos:example "arrow, balls (bullets), blade, cartridges (ammunition cases), gunflints, sling-shot, spear-head"@en ;
  skos:inScheme ocmsot:oc_msotvocab ;
  skos:prefLabel "Weapon"@en ;
.
msot:artifact
  rdf:type skos:Concept ;
  skos:definition "An object made (manufactured, shaped, modified) by a human being, or precursor hominid. Include a set of pieces belonging originally to a single object and treated as a single specimen."@en ;
  skos:inScheme ocmsot:oc_msotvocab ;
  skos:inScheme msot:materialsampleobjecttypevocabulary ;
  skos:prefLabel "Artifact"@en ;
  skos:topConceptOf ocmsot:oc_msotvocab ;
.
msot:organismpart
  rdf:type skos:Concept ;
  skos:definition "Part of an organism, e.g. a tissue sample, plant leaf, flower, bird feather. Include internal parts not composed of organic material (e.g. teeth, bone), and hard body parts that are not shed (hoof, horn, tusk, claw).  Hair is tricky, include here for now.  Does not necessarily imply existance of parent sample. Not fossilized; generally includes organism parts native to deposits of Holocene to Recent age."@en ;
  skos:inScheme ocmsot:oc_msotvocab ;
  skos:inScheme msot:materialsampleobjecttypevocabulary ;
  skos:prefLabel "Organism part"@en ;
  skos:topConceptOf ocmsot:oc_msotvocab ;
.
